DMC3.lean: update

Bakery/DMC3.lean
@@ -5,12 +5,34 @@ universe u
 -- this is merely a marker class i.e. empty fields
 class State (α : Type u) where
 
+abbrev Pattern (α : Type u) [State α] := α → Prop
+
+-- TODO: define ↑ from State to Pattern
+
+-- (inductively defined) set of rules (i.e. Rewrite Theory)
+abbrev Transition (α : Type u) [State α] := α → α → Prop
+
+-- ⊔ for Transition for modular specification
+def joinT {α : Type u} [State α] (t1 t2 : Transition α) : Transition α :=
+  fun st st' => t1 st st' ∨ t2 st st'
+
+-- notation t1 "⊔" t2 => joinT t1 t2 (fix this reserved notation)
+
+
+
+-- Pattern → Pattern → Prop
+abbrev PTransition (α : Type u) [State α] := (α → Prop) → (α → Prop) → Prop
+
+-- (α → α → Prop) → ( (α → Prop) → (α → Prop) → Prop )
+def stepUp {α : Type u} [State α] : Transition α → PTransition α :=
+  fun t => fun p p' => ∀ st st', p st → t st st' → p' st'
+
 --- System: State α with transition relation on α
 class System (α : Type u) [State α] where
   step : α → α → Prop
 
-structure Pattern (α : Type u) [State α] where
-  cond : α → Prop
+-- structure Pattern (α : Type u) [State α] where
+--   cond : α → Prop
 
-def PStep (α : Type u) [State α] [System α] (p : Pattern α) (p' : Pattern α) : Prop :=
-  ∀ st st' : α, p.cond st → System.step st st' → p'.cond st'
+-- def PStep (α : Type u) [State α] [System α] (p : Pattern α) (p' : Pattern α) : Prop :=
+--   ∀ st st' : α, p.cond st → System.step st st' → p'.cond st'
